RelFacts.v
@@ -148,6 +148,7 @@ Module Facts (Sql : SQL).
             apply Rel.T_eqb_eq. reflexivity.
         * apply Rel.p_fs. exact H0.
     + intros. apply Rel.T_eqb_eq. reflexivity.
+
     + intros. apply Rel.T_eqb_eq. reflexivity.
   Qed.
 
@@ -331,9 +332,25 @@ Module Facts (Sql : SQL).
     + extensionality v'. rewrite H0. reflexivity.
   Qed.
 
-  Axiom rsum_id : forall m n (f : Rel.T m -> Rel.R n) r,
+  Lemma rsum_id : forall m n (f : Rel.T m -> Rel.R n) r,
+     m = n ->
      (forall x, f x ~= Rel.Rsingle x) ->
      Rel.rsum r f ~= r.
+  Proof.
+    intros. enough (exists (g : Rel.T m -> Rel.T n), forall x, g x ~= x).
+    decompose record H1. rename x into g; rename H2 into Hg. clear H1.
+    eapply (trans_JMeq _ (sum_id _ _ _ _ H Hg)). Unshelve.
+      subst. exists (fun x => x); intuition.
+    apply eq_JMeq; apply Rel.p_ext. intro.
+    rewrite Rel.p_rsum. rewrite Rel.p_sum.
+    induction (Rel.supp r); intuition.
+    simpl. subst. rewrite H0, Hg, IHl.
+    destruct (Rel.T_dec _ a t).
+    + rewrite e, (proj2 (Rel.T_eqb_eq _ _ _) eq_refl), Rel.p_single. simpl. omega.
+    + enough (Rel.T_eqb a t = false). rewrite H, Rel.p_single_neq. omega.
+      exact n0. destruct (Rel.T_eqb a t) eqn:e. contradiction n0. apply (proj1 (Rel.T_eqb_eq _ _ _)). exact e.
+      reflexivity.
+  Qed.
 
   Lemma Rel_Rone_times n (r : Rel.R n) : Rel.times Rel.Rone r ~= r.
   Proof.
@@ -347,42 +364,394 @@ Module Facts (Sql : SQL).
   Qed.
 
   (* maybe derive from another result: R_sum r (fun Vl => R_single x) = R.sum r (fun Vl => x). *)
-  Axiom rsum_single : forall n (r : Rel.R n), Rel.rsum r (fun Vl => Rel.Rsingle Vl) ~= r.
+  Lemma rsum_single : forall n (r : Rel.R n), Rel.rsum r (fun Vl => Rel.Rsingle Vl) ~= r.
+  Proof.
+    intros. apply rsum_id; intuition.
+  Qed.
+
+(*
+  Lemma memb_sum_tech_r {m} {n} (R : Rel.R m) (f : Rel.T m -> Rel.T n) x l1 : 
+    NoDup l1 -> forall l2, incl l2 (Rel.supp R) -> NoDup l2 -> 
+    (forall t u, List.In t l1 -> List.In u (Rel.supp R) -> List.In t (Rel.supp (f u)) -> List.In u l2) ->
+    (forall u, List.In u l2 -> List.Incl (Rel.supp (f u)) l1) ->
+    list_sum (List.map (fun t => Rel.memb (Rel.rsum R f) t * Rel.memb (g t) x) l1) 
+    = list_sum (List.map (fun u => Rel.memb R u * Rel.memb (Rel.rsum (f t) g) x) l2).
+  Proof.
+    elim l1.
+    + intros. replace l2 with (@List.nil (Rel.T m)). reflexivity.
+      destruct l2; auto. contradiction (H3 t). left. reflexivity.
+    + intros t l1' IH Hl1' l2 Hsupp Hl2 H1 H2. simpl.
+      replace (list_sum (List.map (Rel.memb R) l2)) with
+        (list_sum (List.map (Rel.memb R) (filter (fun x => Rel.T_eqb (f x) t) l2)) +
+         list_sum (List.map (Rel.memb R) (filter (fun x => negb (Rel.T_eqb (f x) t)) l2))).
+      - f_equal.
+        * rewrite Rel.p_sum. apply (list_sum_ext Nat.eq_dec).
+          generalize (Rel.p_nodup _ R) l2 Hsupp Hl2 H1; clear l2 Hsupp Hl2 H1 H2; elim (Rel.supp R).
+          ++ simpl. intros _ l2 Hincl. replace l2 with (@List.nil (Rel.T m)). reflexivity.
+             destruct l2; auto. contradiction (Hincl t0). left. reflexivity.
+          ++ intros x l3' IHin Hnodup l2 Hincl Hl2 H1 y. simpl. destruct (Rel.T_eqb (f x) t) eqn:Heq; simpl.
+            -- destruct (Nat.eq_dec (Rel.memb R x) y); simpl.
+              ** assert (exists n, count_occ Nat.eq_dec 
+                    (List.map (Rel.memb R) (filter (fun x0 : Rel.T m => Rel.T_eqb (f x0) t) l2)) y = S n).
+                  apply count_occ_In_Sn. rewrite <- e. apply in_map. apply filter_In. split; auto.
+                  eapply H1. left. reflexivity. left. reflexivity. apply Rel.T_eqb_eq. exact Heq.
+                destruct H. rewrite (count_occ_rmone_r _ _ _ _ _ H). f_equal.
+                transitivity (count_occ Nat.eq_dec (List.map (Rel.memb R) 
+                  (filter (fun x1 => Rel.T_eqb (f x1) t) (rmone _ (Rel.T_dec _) x l2))) y).
+                +++ apply IHin.
+                  --- inversion Hnodup. exact H4.
+                  --- eapply incl_rmone; assumption.
+                  --- apply nodup_rmone. exact Hl2.
+                  --- intros. apply in_rmone_neq. 
+                    *** inversion Hnodup. intro. rewrite H8 in H6. contradiction H6.
+                    *** eapply H1. exact H0. right. exact H2. exact H3.
+                +++ apply map_filter_tech. exact Heq. rewrite e. reflexivity. 
+                    eapply H1. left. reflexivity. left. reflexivity. apply Rel.T_eqb_eq. exact Heq.
+              ** replace (count_occ Nat.eq_dec (List.map (Rel.memb R) (filter (fun x0 => Rel.T_eqb (f x0) t) l2)) y)
+                  with (count_occ Nat.eq_dec (List.map (Rel.memb R) (filter (fun x0 => Rel.T_eqb (f x0) t) (rmone _ (Rel.T_dec _) x l2))) y).
+                apply IHin.
+                +++ inversion Hnodup. exact H3.
+                +++ eapply incl_rmone; assumption.
+                +++ apply nodup_rmone. exact Hl2. 
+                +++ intros. apply in_rmone_neq. 
+                  --- inversion Hnodup. intro. rewrite H7 in H5. contradiction H5.
+                  --- eapply H1. exact H. right. exact H0. exact H2.
+                +++ apply count_occ_map_filter_rmone_tech. exact n0.
+            -- replace (count_occ Nat.eq_dec (List.map (Rel.memb R) (filter (fun x0 => Rel.T_eqb (f x0) t) l2)) y)
+                  with (count_occ Nat.eq_dec (List.map (Rel.memb R) (filter (fun x0 => Rel.T_eqb (f x0) t) (rmone _ (Rel.T_dec _) x l2))) y). apply IHin.
+              *** inversion Hnodup. exact H3.
+              *** eapply incl_rmone; assumption.
+              *** apply nodup_rmone. exact Hl2. 
+              *** intros. apply in_rmone_neq. 
+                +++ inversion Hnodup. intro. rewrite H7 in H5. contradiction H5.
+                +++ eapply H1. exact H. right. exact H0. exact H2.
+              *** rewrite filter_rmone_false. reflexivity. exact Heq.
+        * apply IH.
+          ++ inversion Hl1'; assumption.
+          ++ intro x. intro Hx. apply Hsupp. 
+             destruct (proj1 (filter_In (fun x => negb (Rel.T_eqb (f x) t)) x l2) Hx). exact H.
+          ++ apply NoDup_filter. exact Hl2.
+          ++ intros. apply filter_In. split.
+            -- eapply H1. right. exact H. exact H0. exact H3.
+            -- apply Bool.negb_true_iff. destruct (Rel.T_dec _ (f u) t).
+              ** inversion Hl1'. rewrite <- e in H6. rewrite H3 in H6. contradiction H6.
+              ** destruct (Rel.T_eqb (f u) t) eqn:ed; auto. contradiction n0. apply Rel.T_eqb_eq. exact ed.
+          ++ intros. assert (List.In u l2 /\ negb (Rel.T_eqb (f u) t) = true).
+            -- apply (proj1 (filter_In (fun x => negb (Rel.T_eqb (f x) t)) u l2) H).
+            -- destruct H0. assert (f u <> t). intro. 
+              pose (H4' := proj2 (Rel.T_eqb_eq _ (f u) t) H4); clearbody H4'.
+              rewrite H4' in H3. discriminate H3. 
+              pose (H2' := H2 _ H0); clearbody H2'. inversion H2'; auto. contradiction H4. symmetry. exact H5.
+      - elim l2; auto.
+        intros x l2' IHin. simpl. destruct (Rel.T_eqb (f x) t); simpl.
+        * rewrite <- IHin. omega.
+        * rewrite <- IHin. omega.
+  Qed.
+
+*)
+
+  Lemma list_sum_plus {A} (f g : A -> nat) l :
+    list_sum (List.map (fun x => f x + g x) l) = list_sum (List.map f l) + list_sum (List.map g l).
+  Proof.
+    induction l; intuition.
+    simpl. rewrite IHl. omega.
+  Qed.
+
+  Lemma list_sum_times_l {A} n (f : A -> nat) l :
+    list_sum (List.map (fun x => n * f x) l) = n * list_sum (List.map f l).
+  Proof.
+    induction l; intuition.
+    simpl. rewrite IHl. rewrite mult_plus_distr_l. reflexivity.
+  Qed.
+
+  Lemma list_sum_append l1 l2 : list_sum (l1 ++ l2) = list_sum l1 + list_sum l2.
+  Proof.
+    induction l1; simpl; intuition.
+  Qed.
+
+  Lemma NoDup_remove {A} (a:A) l1 l2 : NoDup (l1 ++ a :: l2) -> NoDup (l1 ++ l2).
+  Proof.
+    induction l1; simpl; intros.
+    + inversion H; intuition.
+    + constructor. inversion H. intro; apply H2.
+      apply in_or_app. destruct (in_app_or _ _ _ H4).
+      left; assumption. right; right; assumption.
+      apply IHl1. inversion H. intuition.
+  Qed.
+
+  Lemma rsum_rsum_list_sum {A} (l1 l2 : list A) f:
+    NoDup l1 -> NoDup l2 -> incl l2 l1 ->
+    (forall x, List.In x l1 -> ~ List.In x l2 -> f x = 0) ->
+    list_sum (List.map f l1) = list_sum (List.map f l2).
+  Proof.
+    intros. generalize dependent l1; induction l2.
+    + induction l1; simpl; intuition. rewrite H2. apply IHl1. inversion H; intuition.
+      intro. intro. inversion H3.
+      intros. apply H2; intuition. left. reflexivity.
+      intro. inversion H3.
+    + simpl. intros. enough (List.In a l1). decompose record (in_split _ _ H3). rewrite H5.
+      rewrite map_app, list_sum_append. simpl.
+      rewrite (plus_comm (f a)). rewrite plus_assoc. rewrite <- list_sum_append, <- map_app.
+      rewrite plus_comm. f_equal. apply IHl2.
+      - inversion H0; intuition.
+      - rewrite H5 in H. apply (NoDup_remove _ _ _ H).
+      - enough (forall A (y z : A) la lb lc, List.In y la -> y <> z -> incl la (lb ++ z :: lc) -> List.In y (lb ++ lc)).
+        intro. intro. eapply (H4 _ a0 a). apply H6. inversion H0; intro; subst. contradiction H9.
+        intro. intro. enough (List.In a1 (a::l2)).
+        generalize (H1 _ H8). rewrite H5; intuition.
+        right; exact H7.
+        intros B y z la. induction la; simpl; intros. contradiction H4.
+        destruct H4. subst. enough (List.In y (lb ++ z :: lc)).
+        induction lb in H4 |- *; simpl. simpl in H4. destruct H4; subst; intuition.
+        simpl in H4. destruct H4. intuition. right. apply IHlb. exact H4.
+        apply H7. left; reflexivity.
+        apply IHla. exact H4. exact H6. intro. intro. apply H7. right. exact H8.
+      - intros. apply H2. rewrite H5. apply in_or_app. destruct (in_app_or _ _ _  H4).
+        left; exact H7. right; right; exact H7.
+        intro. destruct H7. subst. induction x in H, H4, H3. inversion H. contradiction H5. 
+        apply IHx. simpl in H; inversion H; exact H7.
+        apply in_or_app; right; left; reflexivity.
+        inversion H4. rewrite H1 in H. inversion H. contradiction H7. apply in_or_app; right; left; reflexivity.
+        exact H1.
+        contradiction H6.
+      - apply H1. left; reflexivity.
+  Qed.
+
+  Lemma incl_supp_rsum {m n} a (r : Rel.R m) (f : Rel.T m -> Rel.R n) : 
+    List.In a (Rel.supp r) -> incl (Rel.supp (f a)) (Rel.supp (Rel.rsum r f)).
+  Proof.
+    repeat intro. apply Rel.p_fs. rewrite Rel.p_rsum.
+    generalize (Rel.p_fs_r _ _ _ H0). intro.
+    decompose record (in_split _ _ H). rewrite H3. 
+    rewrite map_app, list_sum_append.
+    replace (list_sum (List.map (fun t0 => Rel.memb r t0 * Rel.memb (f t0) a0) (a :: x0)))
+       with (Rel.memb r a * Rel.memb (f a) a0 + list_sum (List.map (fun t0 => Rel.memb r t0 * Rel.memb (f t0) a0) x0)).
+    2: { reflexivity. }
+    rewrite plus_assoc. rewrite plus_comm. rewrite plus_assoc. change 0 with (0 + 0).
+    apply plus_le_lt_compat. omega.
+    unfold lt. change 1 with (1*1). apply mult_le_compat.
+    apply Rel.p_fs_r. exact H.
+    apply Rel.p_fs_r. exact H0.
+  Qed.
+
+  Lemma rsum_rsum_tech {m n o} (r : Rel.R m) (f : Rel.T m -> Rel.R n) (g : Rel.T n -> Rel.R o) (t : Rel.T o)
+    : forall l, incl l (Rel.supp r) ->
+      list_sum (List.map (fun x =>
+        list_sum (List.map (fun y => 
+          Rel.memb r y * Rel.memb (f y) x) l)
+          * Rel.memb (g x) t) (Rel.supp (Rel.rsum r f))) 
+      = list_sum (List.map (fun z =>
+          Rel.memb r z * list_sum (List.map (fun w => 
+            Rel.memb (f z) w * Rel.memb (g w) t) (Rel.supp (f z)))) l).
+  Proof.
+    induction l; simpl. induction (Rel.supp (Rel.rsum r f)); intuition. intro.
+    transitivity
+      (list_sum (List.map (fun x =>
+        Rel.memb r a * Rel.memb (f a) x * Rel.memb (g x) t
+        + list_sum (List.map (fun y : Rel.T m => Rel.memb r y * Rel.memb (f y) x) l) * Rel.memb (g x) t)
+        (Rel.supp (Rel.rsum r f)))).
+    1: { f_equal. f_equal. extensionality x. rewrite mult_plus_distr_r. reflexivity. }
+    rewrite (list_sum_plus (fun x => Rel.memb r a * Rel.memb (f a) x * Rel.memb (g x) t)
+      (fun x => list_sum (List.map (fun y => Rel.memb r y * Rel.memb (f y) x) l) * Rel.memb (g x) t)).
+    rewrite IHl. f_equal.
+    transitivity (list_sum (List.map (fun x => 
+      Rel.memb r a * (Rel.memb (f a) x * Rel.memb (g x) t)) (Rel.supp (Rel.rsum r f)))).
+    1: { f_equal. f_equal. extensionality x. rewrite mult_assoc. reflexivity. }
+    rewrite (list_sum_times_l (Rel.memb r a) (fun x => Rel.memb (f a) x * Rel.memb (g x) t)).
+    f_equal.
+    apply rsum_rsum_list_sum. apply Rel.p_nodup. apply Rel.p_nodup.
+    apply incl_supp_rsum. apply H. left; reflexivity. 
+    intros. replace (Rel.memb (f a) x) with 0. omega.
+    destruct (or_eq_lt_n_O (Rel.memb (f a) x)). omega.
+    generalize (Rel.p_fs _ _ _ H2). intro. contradiction H1.
+    repeat intro. apply H. right. exact H0.
+  Qed.
 
   Lemma rsum_rsum {m n o} (r : Rel.R m) (f : Rel.T m -> Rel.R n) (g: Rel.T n -> Rel.R o) 
     : Rel.rsum (Rel.rsum r f) g = Rel.rsum r (fun x => Rel.rsum (f x) g).
   Proof.
-    admit.
-  Admitted.
+    apply Rel.p_ext; intro.
+    repeat rewrite Rel.p_rsum.
+    transitivity 
+      (list_sum (List.map (fun x => 
+         list_sum (List.map (fun y => 
+           Rel.memb r y * Rel.memb (f y) x) (Rel.supp r)) 
+         * Rel.memb (g x) t) (Rel.supp (Rel.rsum r f)))).
+    1: { f_equal. f_equal. extensionality x. rewrite Rel.p_rsum. reflexivity. }
+    transitivity
+      (list_sum (List.map (fun z => Rel.memb r z * 
+       list_sum (List.map (fun w => Rel.memb (f z) w * Rel.memb (g w) t) (Rel.supp (f z)))) (Rel.supp r))).
+    2: { f_equal. f_equal. extensionality z. rewrite Rel.p_rsum. reflexivity. }
+    apply rsum_rsum_tech.
+    apply incl_refl.
+  Qed.
 
   Lemma sel_rsum {m n} (r : Rel.R m) (p : Rel.T n -> bool) (f : Rel.T m -> Rel.R n)
     : Rel.sel (Rel.rsum r f) p = Rel.rsum r (fun x => (Rel.sel (f x) p)).
   Proof.
-    admit.
-  Admitted.
+    apply Rel.p_ext; intro. destruct (p t) eqn:ep.
+    + rewrite Rel.p_selt. repeat rewrite Rel.p_rsum.
+      induction (Rel.supp r); intuition.
+      simpl. rewrite Rel.p_selt. intuition. exact ep. exact ep.
+    + rewrite Rel.p_self. rewrite Rel.p_rsum. induction (Rel.supp r); intuition.
+      simpl. rewrite IHl, Rel.p_self. omega. exact ep. exact ep.
+  Qed.
 
   Lemma eq_sum_rsum {m n} r (f : Rel.T m -> Rel.T n) : Rel.sum r f = Rel.rsum r (fun x => Rel.Rsingle (f x)).
   Proof.
-    admit.
-  Admitted.
+    apply Rel.p_ext; intro. rewrite Rel.p_sum, Rel.p_rsum. induction (Rel.supp r); intuition.
+    simpl. destruct (Rel.T_dec _ (f a) t).
+    + rewrite e, (proj2 (Rel.T_eqb_eq _ _ _) eq_refl), Rel.p_single. simpl. omega.
+    + enough (Rel.T_eqb (f a) t = false). rewrite H, Rel.p_single_neq. omega.
+      exact n0. destruct (Rel.T_eqb (f a) t) eqn:e. contradiction n0. apply (proj1 (Rel.T_eqb_eq _ _ _)). exact e.
+      reflexivity.
+  Qed.
 
   Lemma sel_times_single {m n} (r : Rel.R m) (x : Rel.T n) p : 
     Rel.sel (Rel.times r (Rel.Rsingle x)) p = Rel.times (Rel.sel r (fun Vl => p (append Vl x))) (Rel.Rsingle x).
   Proof.
-    admit.
-  Admitted.
+    apply Rel.p_ext; intro. decompose record (exists_vector_append _ _ _ _ t eq_refl). destruct (p t) eqn:ep.
+    + rewrite Rel.p_selt. 
+      repeat rewrite (Rel.p_times _ _ _ _ _ _ _ (JMeq_eq H0)).
+      destruct (Rel.T_dec _ x x1).
+      - subst. rewrite Rel.p_selt. reflexivity. exact ep.
+      - rewrite Rel.p_single_neq. omega. exact n0.
+      - exact ep.
+    + rewrite Rel.p_self. rewrite (Rel.p_times _ _ _ _ _ _ _ (JMeq_eq H0)).
+      destruct (Rel.T_dec _ x x1).
+      - subst. rewrite Rel.p_self. omega. exact ep.
+      - rewrite Rel.p_single_neq. omega. exact n0.
+      - exact ep.
+  Qed.
+
+(*********)
+
+  Lemma filter_false A p (l : list A) : 
+    (forall x, List.In x l -> p x = false) -> filter p l = List.nil.
+  Proof.
+    elim l. auto.
+    intros h t IH Hp. simpl. rewrite Hp.
+    + apply IH. intros. apply Hp. right. exact H.
+    + left. reflexivity.
+  Qed.
+
+  Lemma sum_append : forall m n o (f : Rel.T m -> Rel.T n) r (t : Rel.T o),
+     n = m + o ->
+     (forall x, f x ~= append x t) ->
+     Rel.sum r f ~= Rel.times r (Rel.Rsingle t).
+  Proof.
+    intros. subst. apply eq_JMeq. eapply Rel.p_ext.
+    intros v. rewrite Rel.p_sum.
+    replace (fun x => Rel.T_eqb (f x) v) with (fun v' => Rel.T_eqb (append v' t) v).
+    decompose record (exists_vector_append _ _ _ _ v eq_refl). rename x into v1. rename x0 into v2.
+    rewrite H1, (Rel.p_times _ _ _ _ _ v1 v2 eq_refl).
+    destruct (Rel.T_dec _ t v2).
+    + replace (fun v' => Rel.T_eqb (append v' t) (append v1 v2)) with (fun v' => Rel.T_eqb v' v1).
+      rewrite e, Rel.p_single. eapply filter_supp_elim; simpl; intro.
+      - omega.
+      - destruct (or_eq_lt_n_O (Rel.memb r v1)); intuition.
+        contradiction H. apply Rel.p_fs. exact H2.
+      - extensionality v'. rewrite e. destruct (Rel.T_dec _ v' v1).
+        rewrite (proj2 (Rel.T_eqb_eq _ _ _) e0); symmetry. apply (proj2 (Rel.T_eqb_eq _ _ _)).
+        rewrite e0. reflexivity.
+        replace (Rel.T_eqb v' v1) with false. symmetry.
+        destruct (Rel.T_dec _ (append v' v2) (append v1 v2)). decompose record (vec_append_inj e0).
+        contradiction (n H).
+        destruct (Rel.T_eqb (append v' v2) (append v1 v2)) eqn:eapp.
+        rewrite (proj1 (Rel.T_eqb_eq _ _ _) eapp) in n0. contradiction n0. reflexivity.
+        reflexivity.
+        symmetry. destruct (Rel.T_eqb v' v1) eqn:e0.
+        rewrite (proj1 (Rel.T_eqb_eq _ _ _) e0) in n. contradiction n. reflexivity.
+        reflexivity.
+    + rewrite filter_false. replace (Rel.memb (Rel.Rsingle t) v2) with 0. simpl; omega.
+      rewrite Rel.p_single_neq. reflexivity. exact n.
+      intros v' Hv'. destruct (Rel.T_eqb (append v' t) (append v1 v2)) eqn:eapp.
+      decompose record (vec_append_inj (proj1 (Rel.T_eqb_eq _ _ _) eapp)). contradiction n.
+      reflexivity.
+    + extensionality v'. rewrite H0. reflexivity.
+  Qed.
+
+  Lemma rsum_append : forall m n o (f : Rel.T m -> Rel.R n) r (t : Rel.T o),
+     n = m + o ->
+     (forall x, f x ~= Rel.Rsingle (append x t)) ->
+     Rel.rsum r f ~= Rel.times r (Rel.Rsingle t).
+  Proof.
+    intros; subst. erewrite <- (sum_append _ _ _ (fun x => append x t)).
+    rewrite eq_sum_rsum. replace f with (fun (x:Rel.T m) => Rel.Rsingle (append x t)).
+    reflexivity. extensionality v. rewrite H0. reflexivity.
+    reflexivity.
+    intuition.
+  Qed.
+
+  Lemma supp_single_aux {A} (t : A) (l : list A) :
+    (forall (x y:A), {x = y} + {x <> y}) ->
+    List.In t l ->
+    (forall u, t <> u -> ~ List.In u l) ->
+    NoDup l ->
+    l = t::List.nil.
+  Proof.
+    intros. destruct l.
+    + inversion H.
+    + destruct (X a t).
+      - subst. destruct l; intuition.
+        destruct (X a t); subst.
+        inversion H1. contradiction H4. left. reflexivity.
+        exfalso. apply (H0 a). intuition. right; left; reflexivity.
+      - contradiction (H0 a). intuition. left; reflexivity.
+  Qed.
+
+  Lemma supp_single : forall n (t : Rel.T n), Rel.supp (Rel.Rsingle t) = t::List.nil.
+  Proof.
+    intros. apply supp_single_aux. apply (Rel.T_dec _).
+    apply Rel.p_fs. rewrite Rel.p_single. omega.
+    intros. intro. generalize (Rel.p_fs_r _ _ _ H0). rewrite Rel.p_single_neq. omega.
+    assumption.
+    apply Rel.p_nodup.
+  Qed.
+
+  Lemma rsum_from_single : forall m n t (f : Rel.T m -> Rel.R n), 
+    Rel.rsum (Rel.Rsingle t) f = f t.
+  Proof.
+    intros. apply Rel.p_ext. intro. rewrite Rel.p_rsum.
+    replace (Rel.supp (Rel.Rsingle t)) with (t::List.nil).
+    simpl. rewrite Rel.p_single. omega.
+    symmetry; apply supp_single.
+  Qed.
 
   Lemma rsum_times_single {m n o} (r : Rel.R m) (x : Rel.T n) (f : Rel.T (m + n) -> Rel.R o) :
     Rel.rsum (Rel.times r (Rel.Rsingle x)) f = Rel.rsum r (fun Vl => f (append Vl x)).
   Proof.
-    admit.
-  Admitted.
+    replace (Rel.times r (Rel.Rsingle x)) with (Rel.rsum r (fun v => Rel.Rsingle (append v x))).
+    rewrite rsum_rsum. f_equal.
+    extensionality Vl. apply rsum_from_single.
+    apply JMeq_eq. apply rsum_append. reflexivity. intuition.
+  Qed.
+
+  Lemma flatnat_plus : forall x y, Rel.flatnat (x + y) = max (Rel.flatnat x) (Rel.flatnat y).
+  Proof.
+    intros. destruct x; destruct y; simpl; reflexivity.
+  Qed.
+
+  Lemma flatnat_times : forall x y, Rel.flatnat (x * y) = min (Rel.flatnat x) (Rel.flatnat y).
+  Proof.
+    intros. destruct x; destruct y; simpl; intuition.
+    replace (x * 0) with 0. reflexivity. omega.
+  Qed.
+
+  Lemma flatnat_flatnat : forall x, Rel.flatnat (Rel.flatnat x) = Rel.flatnat x.
+  Proof.
+    intros. destruct x; reflexivity.
+  Qed.
 
   Lemma flat_rsum_flat {m n} (r : Rel.R m) (fr : Rel.T m -> Rel.R n) : 
     Rel.flat (Rel.rsum r (fun Vl => Rel.flat (fr Vl))) = Rel.flat (Rel.rsum r (fun Vl => fr Vl)).
   Proof.
-    admit.
-  Admitted.
+    apply Rel.p_ext; intro. repeat rewrite Rel.p_flat. repeat rewrite Rel.p_rsum.
+    induction (Rel.supp r); intuition.
+    simpl. repeat rewrite flatnat_plus. rewrite IHl. f_equal.
+    rewrite Rel.p_flat. repeat rewrite flatnat_times. f_equal.
+    apply flatnat_flatnat.
+  Qed.
 
   Lemma flat_Rsingle n (v : Rel.T n) : Rel.flat (Rel.Rsingle v) = Rel.Rsingle v.
   Proof.
@@ -393,6 +762,24 @@ Module Facts (Sql : SQL).
   Qed.
 
   Lemma sum_Rone_Rsingle n (f : Rel.T 0 -> Rel.T n) : Rel.sum Rel.Rone f = Rel.Rsingle (f (Vector.nil _)).
-  Proof. admit. Admitted.
+  Proof.
+    apply Rel.p_ext; intro. rewrite Rel.p_sum. replace (Rel.supp Rel.Rone) with (Vector.nil Rel.V ::List.nil).
+    destruct (Rel.T_dec _ (f (nil _)) t).
+    + rewrite e. rewrite Rel.p_single. 
+      simpl. rewrite e. simpl. rewrite (proj2 (Rel.T_eqb_eq _ _ _) eq_refl). simpl. rewrite Rel.p_one. omega.
+    + rewrite Rel.p_single_neq. simpl. destruct (Rel.T_eqb (f (nil _)) t) eqn:e; simpl; intuition.
+      contradiction n0. apply Rel.T_eqb_eq. exact e. exact n0.
+    + enough (forall x y z, Rel.supp Rel.Rone <> x::y::z).
+      enough (Rel.supp Rel.Rone <> List.nil).
+      destruct (Rel.supp Rel.Rone). contradiction H0. reflexivity.
+      destruct l. eapply (Vector.case0 (fun x => _ = x :: _)). reflexivity.
+      contradiction (H t0 t1 l). reflexivity.
+      intro. enough (List.In (nil _) (Rel.supp Rel.Rone)). rewrite H0 in H1; exact H1.
+      apply Rel.p_fs. rewrite Rel.p_one. omega.
+      intros. intro. generalize (Rel.p_nodup _ Rel.Rone).
+      rewrite H. eapply (Vector.case0 (fun a => NoDup (a :: _) -> False)).
+      eapply (Vector.case0 (fun a => NoDup (_ :: a :: _) -> False)). intro.
+      inversion H0. contradiction H3. simpl. left. reflexivity.
+  Qed.
 
 End Facts.
